Removed the char_t def and changed uses of char_t to char_p.
Moved def of Alphabet.v to ParserArg.v and removed Alphabet.v.

x86model/Model/ParserArg.v
@@ -2,6 +2,9 @@ Require Import Bool.
 Require Import ZArith.
 Require Import List.
 
+Require Import String.
+Require Import Structures.OrdersAlt.
+
 Module Type PARSER_ARG.
   (* the type of characters used in the grammar specifications *)
   Parameter char_p : Set.
@@ -9,6 +12,12 @@ Module Type PARSER_ARG.
      paired with a proof that it's an equality so that
      we get faster symbolic computation. *)
   Parameter char_dec : forall (c1 c2:char_p), {c1=c2} + {c1<>c2}.
+  
+  (* compare two chars *)
+  Parameter char_cmp : char_p -> char_p -> comparison.
+  Parameter char_eq_leibniz :
+    forall c1 c2, char_cmp c1 c2 = Eq -> c1 = c2.
+
   (* a name for user types embedded within our AST grammar types. *)
   Parameter user_type : Set.
   (* equality on user type names. *)
@@ -18,7 +27,7 @@ Module Type PARSER_ARG.
 
   (* when we parse, instead of working in terms of individual characters,
      we work in terms of tokens.   For instance, the x86 grammar is specified
-     with characters as bits, and tokens as bytes (8-bits. *)
+     with characters as bits, and tokens as bytes (8-bits). *)
   Definition token_id := nat.
   (* this is the total number of tokens that we can have -- e.g., for the
      x86 parser it is 256 because they have 8 bits. *)
@@ -26,7 +35,12 @@ Module Type PARSER_ARG.
   (* this converts tokens to a list of characters -- it's used only during
      the table construction for the parser. *)
   Variable token_id_to_chars : token_id -> list char_p.
+
+  (* converts a char to a string *)
+  Parameter show_char: char_p -> string.
+
 End PARSER_ARG.
+
 
 (* a module for generating the parser for x86 instructions *)
 Module X86_PARSER_ARG.
@@ -103,6 +117,20 @@ Module X86_PARSER_ARG.
       | Option_t t => option (tipe_m t)
       | UPair_t t1 t2 => ((tipe_m t1) * (tipe_m t2))%type
     end.
+
+  Definition char_cmp (c1 c2:char_p) : comparison :=
+    match c1, c2 with
+      | false, true => Lt
+      | true, false => Gt
+      | _, _ => Eq
+    end.
+
+  Lemma char_eq_leibniz :
+    forall c1 c2, char_cmp c1 c2 = Eq -> c1 = c2.
+  Proof.
+    destruct c1 ; destruct c2 ; intros  ; auto ; discriminate.
+  Qed.
+
   Definition user_type := type.
   Definition user_type_dec : forall (t1 t2:user_type), {t1=t2} + {t1<>t2} := 
     tipe_eq.
@@ -118,7 +146,36 @@ Module X86_PARSER_ARG.
   Definition token_id := nat.
   Definition num_tokens : token_id := 256%nat.
   Definition token_id_to_chars : token_id -> list char_p := nat_explode.
+
+  Open Scope string_scope.
+  Definition show_char (c:char_p) : string :=
+    match c with
+      | true => "1"
+      | false => "0"
+    end.
+
 End X86_PARSER_ARG.
+
+Require Import Coq.Structures.OrdersAlt.
+Module CharOrderedTypeAlt <: OrderedTypeAlt.
+  Definition t : Type := X86_PARSER_ARG.char_p.
+  Definition compare : t -> t -> comparison := X86_PARSER_ARG.char_cmp.
+
+  Lemma compare_sym : forall (c1 c2 : t), compare c2 c1 = CompOpp (compare c1 c2).
+  Proof.
+    destruct c1 ; destruct c2 ; auto.
+  Qed.
+
+  Lemma compare_trans :
+    forall cmp c1 c2 c3, compare c1 c2 = cmp  -> compare c2 c3 = cmp -> compare c1 c3 = cmp.
+  Proof.
+    destruct c1 ; destruct c2 ; destruct c3 ; simpl ; intros ; subst ; auto ; discriminate.
+  Qed.
+End CharOrderedTypeAlt.
+
+Module CharOrderedType := OT_from_Alt CharOrderedTypeAlt.
+
+
 
 (******************************************************************************)
 (* I would like to put this in a module but alas, the Extraction Implicit     *)
